[minor] Progress on a hello world program

sealing/main.v
@@ -6,8 +6,11 @@ Require Import lib.utils lib.partial_maps common.common.
 Require Import concrete.concrete.
 Require Import concrete.int_32.
 Require Import symbolic.int_32.
+Require Import sealing.symbolic.
 Require Import symbolic.fault_handler.
 Require Import sealing.abstract.
+Require Import concrete.exec.
+Require Import Integers.
 Require Import Omega.
 
 Set Implicit Arguments.
@@ -81,6 +84,27 @@ Instance ap : Abs.params t := {|
 |}.
 *)
 
+Instance cp : Concrete.concrete_params t := {|
+  memory    := Int32PMap.t atom;
+  registers := Int32TMap.t atom;
+
+  mem_class := {|
+    PartMaps.get mem i := Int32PMap.get i mem;
+    PartMaps.set mem i x := Int32PMap.set i x mem;
+    PartMaps.upd mem i x := match Int32PMap.get i mem with
+                              | Some _ => Some (Int32PMap.set i x mem)
+                              | None   => None
+                            end
+  |};
+
+  reg_class := {|
+    TotalMaps.get regs r := Int32TMap.get r regs;
+    (* BCP/MD: Why isn't this called 'set'? *)
+    TotalMaps.upd regs r x := Int32TMap.set r x regs
+  |}
+|}.
+
+
 (* Need to build...
 
    - encoding of tags
@@ -112,40 +136,68 @@ Instance ap : Abs.params t := {|
 (* ---------------------------------------------------------------- *)
 (* Code combinators... *)
 
-Definition constant_code (l : list atom) : @relocatable_segment t w atom := 
-  (length l, fun _ _ => l).
+Definition constant_data l : @relocatable_segment t w atom := 
+  (length l, fun _ _ => map (fun x => Atom x Concrete.TKernel) l).
+
+Definition make_code l :=
+  map (fun x => Atom (encode_instr x) Concrete.TKernel) l.
+
+Definition constant_code {X} l : @relocatable_segment t X atom := 
+  (length l, fun _ _ => make_code l).
 
 (* ---------------------------------------------------------------- *)
 (* Main definitions *)
 
-Axiom fault_handler : @relocatable_segment t w atom. 
+(* Axiom fault_handler : @relocatable_segment t w atom.  *)
 
-(*
-Axiom transfer_function : instr list.
+Definition transfer_function : list (instr t) :=
+  [].
+(* TODO *)
 
 Definition fault_handler : @relocatable_segment t w atom :=
-  constant_code (handler transfer_function)
-.
-*)
+  constant_code (handler t ops fhp transfer_function).
 
 Definition extra_state : @relocatable_segment t w atom := 
-  constant_code [Atom (nat_to_word 0) Concrete.TKernel].
+  constant_data [nat_to_word 0].
 
-Axiom mkkey_segment : @relocatable_segment t w atom.
-(*
+Instance sk_defs : Sym.sealing_key := {|
+  key := int_eqType;
+  max_key := Int32.repr 100;
+  inc_key := fun x => Int32.add x (Int32.repr 1);
+  ord_key := int_ordered
+|}.
+Admitted.
+
+Definition encode_sealing_tag (t : Sym.stag) : w := 
+  match t with
+    Sym.DATA => Z_to_word 0
+  | Sym.KEY k => Z_to_word 1     (* TODO FIX *)
+  | Sym.SEALED k => Z_to_word 2
+  end.
+
 Definition mkkey_segment : @relocatable_segment t w atom :=
-  (2, fun _ (extra : w) => [
-          Const t (word_to_imm extra) (ri t);
-          Load t (ri t) (ri t)
+  (2, fun _ (extra : w) => make_code [
+          (* TODO: too many numeric types! *)
+          Const _ (Z_to_imm (word_to_Z extra)) (ri1 t);
+          Load _ (ri1 t) (ri2 t);
+          (* TODO: More here! *)
+          Jump _ (rra t)
           ]).
-*)
 
-Axiom seal_segment : @relocatable_segment t w atom.
-Axiom unseal_segment : @relocatable_segment t w atom.
+Definition seal_segment : @relocatable_segment t w atom :=
+  (2, fun _ (extra : w) => make_code [
+          (* TODO: More here! *)
+          Jump _ (rra t)
+          ]).
+
+Definition unseal_segment : @relocatable_segment t w atom :=
+  (2, fun _ (extra : w) => make_code [
+          (* TODO: More here! *)
+          Jump _ (rra t)
+          ]).
 
 Definition build_concrete_sealing_machine 
      (user_mem : @relocatable_segment t unit atom) 
-     (initial_pc_tag : w)   (* Doesn't make sense for sealing *)
    : Concrete.state concrete_int_32_t :=
   let syscalls :=
     concat_relocatable_segments
@@ -157,7 +209,51 @@ Definition build_concrete_sealing_machine
     extra_state
     handler_and_syscalls
     (@relocate_ignore_args t w atom user_mem)
-    initial_pc_tag.
+    (encode_sealing_tag Sym.DATA).
+
+Definition hello_world : @relocatable_segment t unit atom :=
+  constant_code [
+    Const _ (Z_to_imm 2) (ri1 t);
+    Binop _ ADD (ri2 t) (ri2 t) (ri3 t)
+  ].
+
+Definition trivial_masks : Concrete.Masks :=
+  fun _ _ => {|
+    Concrete.dc := fun _ => false;
+    Concrete.ct := {| Concrete.ct_trpc := None; 
+                      Concrete.ct_tr := None |}
+  |}.
+
+End WithClasses.
+
+Instance scr : @syscall_regs t := {|
+  syscall_ret  := Int32.repr 20;
+  syscall_arg1 := Int32.repr 21;
+  syscall_arg2 := Int32.repr 22
+|}.
+
+(* BCP/MD: There should be some proof obligations about -- at least --
+   these being pairwise distinct.  Some axioms must be false
+   somewhere! *)
+Instance fhp : fault_handler.fault_handler_params t := {|
+  rop := Int32.repr 1; 
+  rtpc := Int32.repr 2; 
+  rti := Int32.repr 3; rt1 := Int32.repr 4; rt2 := Int32.repr 5; 
+  rt3 := Int32.repr 6; 
+  rb := Int32.repr 7; 
+  ri1 := Int32.repr 8; ri2 := Int32.repr 9; ri3 := Int32.repr 10; 
+  ri4 := Int32.repr 11; ri5 := Int32.repr 12; 
+  rtrpc := Int32.repr 13; rtr := Int32.repr 14; 
+  raddr := Int32.repr 15; 
+  rra := Int32.repr 16;
+
+  load_const := fun (x : word t) (r : reg t) =>
+    [Const _ (Z_to_imm (word_to_Z x)) r]
+|}.
+
+(*
+Goal exec.step trivial_masks t (build_concrete_sealing_machine hello_world) = None.
+*)
 
 (* BCP: One nontrivial issue here.  How do we find out the system call
 addresses to use when instantiating the sealing machine?
@@ -172,5 +268,4 @@ Definition build_abstract_sealing_machine :=
 
 (* TODO: Refinement proof from concrete to abstract instances *)
 
-End WithClasses.
 End ConcreteSealing.
